theories/host.v
@@ -14,31 +14,33 @@ Variable host_function : Type.
 Let store_record := store_record host_function.
 
 (** The application of a host function either:
-  - returns a result [Some (st', result)], containing a new store and a result (which can be [Trap]),
+  - returns [Some (st', result)], returning a new Wasm store and a result (which can be [Trap]),
   - diverges, represented as [None].
   This can be non-deterministic. **)
 
 (** We provide two versions of the host.
-  One computable based on the [host_apply] monadic binder, to be used in the interpreter,
-  and one based on a relation, to be used in the operational semantics. **)
-
-Record monadic_host := {
-    host_monad : Type -> Type ;
-    host_return : forall A, A -> host_monad A ;
-    host_bind : forall A B, host_monad A -> (A -> host_monad B) -> host_monad B ;
-    host_apply :
-      store_record -> host_function -> seq value ->
-      host_monad (option (store_record * result)) ;
-    (* FIXME: Should it be defined after the typing, to get some notions of correctness? *)
-  }.
+  One based on a relation, to be used in the operational semantics,
+  and one computable based on the [host_monad] monad, to be used in the interpreter.
+  There is no host state in the host monad: it is entirely caught by the (state) monad. **)
 
 Record host := {
     host_state : eqType ;
     host_application : host_state -> store_record -> host_function -> seq value ->
                        host_state -> option (store_record * result) -> Prop
+    (* FIXME: Should the resulting [host_state] be part of the [option]? *)
   }.
 
-(* TODO: Relation between [monadic_host] and [host]. *)
+Record monadic_host := {
+    host_monad : Type -> Type ;
+    host_return : forall A, A -> host_monad A ;
+    host_bind : forall A B, host_monad A -> (A -> host_monad B) -> host_monad B ;
+    host_apply : store_record -> host_function -> seq value ->
+                 host_monad (option (store_record * result))
+  }.
+
+(** Relation between [monadic_host] and [host]. **)
+
+(* TODO *)
 
 End Parameterised.
 
